killing admit of SteelAtomic.frame0

pulse/ulib/experimental/Steel.Effect.Atomic.fst
@@ -141,27 +141,54 @@ let atomic_preserves_frame_and_preorder
 #pop-options
 
 #push-options "--fuel 0 --ifuel 0 --z3rlimit 10"
-// let frame0 (#a:Type) (#uses:Set.set lock_addr) (#is_ghost:bool) (#pre:pre_t) (#post:post_t a)
-//   (f:atomic_repr a uses is_ghost pre post)
-//   (frame:hprop)
-// : SteelAtomic a
-//   uses
-//   is_ghost
-//   (pre `star` frame)
-//   (fun x -> post x `star` frame)
-// = admit ()
 
-// SteelAtomic?.reflect (fun _ ->
-//     //let m0 = NMSTTotal.get () in
-//     let x = f () in
-//     x)
+let frame_repr_raw (#a:Type) (#uses:Set.set lock_addr) (#is_ghost:bool) (#pre:pre_t) (#post:post_t a)
+    (f:atomic_repr a uses is_ghost pre post)
+    (frame:hprop)
+    (_:unit)
+  : MstTot a
+      (requires fun m0 ->
+        let open Sem in
+        let st = state_uses uses in
+        st.interp ((pre `st.star` frame) `st.star` st.locks_invariant m0) m0)
+      (ensures fun m0 x m1 ->
+        let open Sem in
+        let st = state_uses uses in
+        st.interp ((post x `st.star` frame) `st.star` st.locks_invariant m1) m1 /\
+        Sem.preserves_frame #st (pre `st.star` frame) (post x `st.star` frame) m0 m1)
+ = let open Sem in
+   let st = state_uses uses in
+   let m0 = mst_get() in
+   let x = f () in
+   let m1 = mst_get() in
+   assert (preserves_frame #st pre (post x) m0 m1);
+   assert (st.interp (post x `st.star` st.locks_invariant m1) m1);
+   assert (st.interp (post x) m1);
+   assert (st.interp (post x `st.star` frame) m1);
+   assert (st.interp ((post x `st.star` frame) `st.star` st.locks_invariant m1) m1);
+   Sem.preserves_frame_star #st pre (post x) m0 m1 frame;
+   assert (preserves_frame #st (pre `st.star` frame) (post x `st.star` frame) m0 m1);
+   x
 
 
+let frame_repr (#a:Type) (#uses:Set.set lock_addr) (#is_ghost:bool) (#pre:pre_t) (#post:post_t a)
+    (f:atomic_repr a uses is_ghost pre post)
+    (frame:hprop)
+  : atomic_repr a uses is_ghost (pre `star` frame) (fun x -> post x `star` frame)
+  = frame_repr_raw f frame
 
-// Sem.run #(state_uses uses) #_ #_ #_ #_ #_ (Sem.Frame (Sem.Act f) frame (fun _ -> True)))
+let frame0 (#a:Type) (#uses:Set.set lock_addr) (#is_ghost:bool) (#pre:pre_t) (#post:post_t a)
+  (f:atomic_repr a uses is_ghost pre post)
+  (frame:hprop)
+: SteelAtomic a
+  uses
+  is_ghost
+  (pre `star` frame)
+  (fun x -> post x `star` frame)
+= SteelAtomic?.reflect (frame_repr f frame)
 #pop-options
 
-assume val  atomic_frame (#a:Type) (#uses:Set.set lock_addr) (#is_ghost:bool) (#pre:pre_t) (#post:post_t a)
+let atomic_frame (#a:Type) (#uses:Set.set lock_addr) (#is_ghost:bool) (#pre:pre_t) (#post:post_t a)
   (frame:hprop)
   ($f:unit -> SteelAtomic a uses is_ghost pre post)
 : SteelAtomic a
@@ -169,7 +196,7 @@ assume val  atomic_frame (#a:Type) (#uses:Set.set lock_addr) (#is_ghost:bool) (#
   is_ghost
   (pre `star` frame)
   (fun x -> post x `star` frame)
-// = admit () //frame0 (reify (f ())) frame
+= frame0 (reify (f ())) frame
 
 let inv_witnessed (#p:hprop) (i:inv p) =
   NMSTTotal.witnessed mem mem_evolves (inv_ok i)
